split lgraph/liso from pttdom.v

coq/pttdom.v
@@ -1,6 +1,6 @@
-Require Import Setoid CMorphisms Morphisms.
+Require Import Setoid CMorphisms.
 From mathcomp Require Import all_ssreflect.
-Require Import edone finite_quotient preliminaries bij equiv multigraph_new.
+Require Import edone finite_quotient preliminaries bij equiv multigraph_new liso.
 
 Set Implicit Arguments.
 Unset Strict Implicit.
@@ -74,288 +74,6 @@ Lemma merge43E':
    (merge43^-1 None = \pi inl true) *
    (merge43^-1 (Some true) = \pi inr true))%type.
 Admitted.
-
-(** 2pdom terms  *)
-
-Inductive term :=
-| dot: term -> term -> term
-| par: term -> term -> term
-| cnv: term -> term
-| dom: term -> term
-| one: term
-| var: sym -> term.
-
-Bind Scope pttdom_ops with term.
-Open Scope pttdom_ops.
-Notation "x ∥ y" := (par x y) (left associativity, at level 25, format "x ∥ y"): pttdom_ops.
-Notation "x · y" := (dot x y) (left associativity, at level 20, format "x · y"): pttdom_ops.
-Notation "x °"  := (cnv x) (left associativity, at level 5, format "x °"): pttdom_ops.
-Notation "1"  := (one): pttdom_ops.
-
-Reserved Notation "x ≡ y" (at level 79).
-
-(** 2pdom axioms  *)
-(* NOTE: the 2pdom axioms are listed here, while the rest of the code is for 2p + TaT=T
-   (to be fixed later)
- *)
-
-Inductive weq: relation term :=
-| weq_refl: Reflexive weq
-| weq_trans: Transitive weq
-| weq_sym: Symmetric weq
-| dot_weq: Proper (weq ==> weq ==> weq) dot
-| par_weq: Proper (weq ==> weq ==> weq) par
-| cnv_weq: Proper (weq ==> weq) cnv
-| dom_weq: Proper (weq ==> weq) dom
-| parA: forall x y z, x ∥ (y ∥ z) ≡ (x ∥ y) ∥ z
-| parC: forall x y, x ∥ y ≡ y ∥ x
-| dotA: forall x y z, x · (y · z) ≡ (x · y) · z
-| dotx1: forall x, x · 1 ≡ x
-| cnvI: forall x, x°° ≡ x
-| cnvpar: forall x y, (x ∥ y)° ≡ x° ∥ y°
-| cnvdot: forall x y, (x · y)° ≡ y° · x°
-| par11: 1 ∥ 1 ≡ 1
-| A10: forall x y, 1 ∥ x·y ≡ dom (x ∥ y°)
-| A13: forall x y, dom (x·y) ≡ dom (x·dom y)
-| A14: forall x y z, dom x·(y ∥ z) ≡ dom x · y ∥ z
-where "x ≡ y" := (weq x y).
-
-Instance Equivalence_weq: Equivalence weq.
-Proof. split. apply weq_refl. apply weq_sym. apply weq_trans. Qed.
-Existing Instance dot_weq.
-Existing Instance par_weq.
-Existing Instance cnv_weq.
-Existing Instance dom_weq.
-
-Canonical Structure term_setoid := Setoid Equivalence_weq.
-
-(** * tests *)
-
-Fixpoint is_test (u: term) :=
-  match u with
-  | dot u v => is_test u && is_test v
-  | par u v => is_test u || is_test v
-  | cnv u => is_test u
-  | dom _ | one => true
-  | var _ => false
-  end.
-
-Record test := Test{ term_of:> term ; testE: is_test term_of }.
-Definition infer_test x y (e: term_of y = x) := y.
-Notation "[ x ]" := (@infer_test x _ erefl).
-
-Canonical Structure tst_one := @Test 1 erefl. 
-Canonical Structure tst_dom u := @Test (dom u) erefl.
-Lemma par_test (a: test) (u: term): is_test (a∥u).
-Proof. by rewrite /=testE. Qed.
-Canonical Structure tst_par a u := Test (par_test a u). 
-Lemma dot_test (a b: test): is_test (a·b).
-Proof. by rewrite /=2!testE. Qed.
-Canonical Structure tst_dot a b := Test (dot_test a b).
-Lemma cnv_test (a: test): is_test (a°).
-Proof. by rewrite /=testE. Qed.
-Canonical Structure tst_cnv a := Test (cnv_test a).
-
-Lemma dotC (a b: test): a·b ≡ b·a.
-Admitted.
-
-Definition test_weq (a b: test) := a ≡ b.
-Instance Equivalence_test_weq: Equivalence test_weq.
-Admitted.
-Canonical Structure test_setoid := Setoid Equivalence_test_weq.
-Instance test_monoid: comm_monoid test_setoid :=
-  { mon0 := [1];
-    mon2 a b := [a·b] }.
-  by intros ??????; apply dot_weq.
-  by intros ???; apply dotA.
-  apply dotC.   
-  by intros ?; apply dotx1.
-Defined.
-
-
-(** * normalisation  *)
-
-Inductive nf_term :=
-| nf_test: test -> nf_term
-| nf_conn: test -> term -> test -> nf_term.
-
-Definition term_of_nf (t: nf_term): term :=
-  match t with
-  | nf_test alpha => alpha
-  | nf_conn alpha u gamma => alpha · u · gamma
-  end.                                         
-
-Definition nf_one := nf_test [1].
-Definition nf_var a := nf_conn [1] (var a) [1].
-Definition nf_cnv u :=
-  match u with
-  | nf_test _ => u
-  | nf_conn a u b => nf_conn b (u°) a
-  end.
-Definition nf_dom u :=
-  match u with
-  | nf_test _ => u
-  | nf_conn a u b => nf_test [a · dom (u·b)]
-  end.
-Definition nf_dot u v :=
-  match u,v with
-  | nf_test a, nf_test b => nf_test [a·b]
-  | nf_test a, nf_conn b u c => nf_conn [a·b] u c
-  | nf_conn a u b, nf_test c => nf_conn a u [b·c]
-  | nf_conn a u b, nf_conn c v d => nf_conn a (u·b·c·v) d
-  end.
-Definition nf_par u v :=
-  match u,v with
-  | nf_test a, nf_test b => nf_test [a·b]
-  | nf_test a, nf_conn b u c => nf_test [a ∥ b·u·c]
-  | nf_conn a u b, nf_test c => nf_test [c ∥ a·u·b]
-  | nf_conn a u b, nf_conn c v d => nf_conn [a·c] (u ∥ v) [b·d]
-  end.
-Fixpoint nf (u: term): nf_term :=
-  match u with
-  | dot u v => nf_dot (nf u) (nf v)
-  | par u v => nf_par (nf u) (nf v)
-  | cnv u => nf_cnv (nf u) 
-  | var a => nf_var a
-  | dom u => nf_dom (nf u)
-  | one => nf_one
-  end.
-
-Proposition nf_correct (u: term): u ≡ term_of_nf (nf u).
-Proof.
-  induction u=>//=.
-  - rewrite {1}IHu1 {1}IHu2.
-    case (nf u1)=>[a|a u b];
-    case (nf u2)=>[c|c v d]=>//=; 
-    rewrite !dotA//.
-  - rewrite {1}IHu1 {1}IHu2.
-    case (nf u1)=>[a|a u b];
-    case (nf u2)=>[c|c v d]=>//=.
-    admit.                      (* ok *)
-    apply parC.
-    admit.                      (* ok *)
-  - rewrite {1}IHu.
-    case (nf u)=>[a|a v b]=>//=.
-    admit.                      (* ok *)
-    rewrite 2!cnvdot dotA.
-    admit. (* ok *)
-  - rewrite {1}IHu.
-    case (nf u)=>[a|a v b]=>//=.
-    admit.                      (* ok *)
-    admit.                      (* ok *)
-  - rewrite dotx1.
-    admit.                      (* ok *)
-Admitted.
-
-
-(** * term labelled two-pointed graphs *)
-
-Record lgraph :=
-  LGraph { graph_of :> graph test_setoid term_setoid;
-           input : vertex graph_of;
-           output : vertex graph_of}.
-Arguments input [_].
-Arguments output [_].
-Notation point G := (@LGraph G).
-
-Definition label (G: lgraph) (x: vertex G + edge G): term :=
-  match x with inl v => vlabel v | inr e => elabel e end.
-
-Definition cnv' (b: bool) (u: term): term :=
-  if b then u° else u.
-Definition elabel' (G: lgraph) (b: bool) (e: edge G): term :=
-  cnv' b (elabel e).
-Definition source' (G: lgraph) (b: bool) (e: edge G): G :=
-  if b then target e else source e.
-Definition target' (G: lgraph) (b: bool) (e: edge G): G :=
-  if b then source e else target e.
-
-Definition mkLGraph (V : finType) (E : finType) (s t : E -> V) 
-                    (lv : V -> test_setoid) (le : E -> term_setoid) (i o : V) := point (Graph s t lv le) i o.
-
-Import CMorphisms.
-
-Universe L.
-Record liso (F G: lgraph): Type@{L} :=
-  Liso {
-      liso_v:> bij F G;
-      liso_e: bij (edge F) (edge G);
-      liso_dir: edge F -> bool;
-      vlabel_liso: forall v, term_of (vlabel (liso_v v)) ≡ vlabel v;
-      elabel_liso: forall e, elabel' (liso_dir e) (liso_e e) ≡ elabel e;
-      source_liso: forall e, source' (liso_dir e) (liso_e e) = liso_v (source e);
-      target_liso: forall e, target' (liso_dir e) (liso_e e) = liso_v (target e);
-      liso_input: liso_v input = input;
-      liso_output: liso_v output = output }.
-
-Notation "h '.e'" := (liso_e h) (at level 2, left associativity, format "h '.e'"). 
-Notation "h '.d'" := (liso_dir h) (at level 2, left associativity, format "h '.d'"). 
-
-(* TOMOVE (first one) *)
-Tactic Notation "iso" uconstr(h) uconstr(k) :=
-  match goal with |- iso ?G ?H => apply (@Iso _ _ G H h k) end.
-Tactic Notation "liso" uconstr(h) uconstr(k) uconstr(d) :=
-  match goal with |- liso ?G ?H => apply (@Liso G H h k d) end.
-
-Lemma src_tgt_liso (F G: lgraph) (h: liso F G) e:
- (  (source' (liso_dir h e) (liso_e h e) = liso_v h (source e))
-  * (target' (liso_dir h e) (liso_e h e) = liso_v h (target e)))%type.
-Proof. split; apply h. Qed.
-
-Definition liso_id {G: lgraph}: liso G G.
-  exists bij_id bij_id (fun _ => false)=>//.
-Defined.
-Definition liso_comp F G H (f: liso F G) (g: liso G H): liso F H.
-  exists (bij_comp f g) (bij_comp (liso_e f) (liso_e g))
-       (fun e => liso_dir f e != liso_dir g (liso_e f e))=>//=.
-  move=>v. by rewrite->2vlabel_liso.
-  move=>e. generalize (elabel_liso f e). generalize (elabel_liso g (liso_e f e)).
-  by case liso_dir; case liso_dir=>/= E E'; rewrite<-E',<-E,?cnvI.
-  move=>e. generalize (src_tgt_liso f e). generalize (src_tgt_liso g (liso_e f e)).
-  by case liso_dir; case liso_dir=>/= E E'; rewrite -E' -E.
-  move=>e. generalize (src_tgt_liso f e). generalize (src_tgt_liso g (liso_e f e)).
-  by case liso_dir; case liso_dir=>/= E E'; rewrite -E' -E.
-  by rewrite->2liso_input. 
-  by rewrite->2liso_output.
-Defined.
-Definition liso_sym F G (f: liso F G): liso G F.
-  exists (bij_sym f) (bij_sym (liso_e f))
-       (fun e => liso_dir f ((liso_e f)^-1 e))=>//=.
-  move=>v. rewrite<-(bijK' f v) at 2. by rewrite->vlabel_liso.
-  move=>e. generalize (elabel_liso f ((liso_e f)^-1 e)) =>/=. rewrite bijK'.
-  case liso_dir=>/=E. by rewrite <-E, cnvI. by symmetry. 
-  move=>e. generalize (src_tgt_liso f ((liso_e f)^-1 e)) =>/=. rewrite bijK'. 
-  case liso_dir=>/=E; by apply (@bij_injective _ _ f); rewrite bijK' -E.
-  move=>e. generalize (src_tgt_liso f ((liso_e f)^-1 e)) =>/=. rewrite bijK'. 
-  case liso_dir=>/=E; by apply (@bij_injective _ _ f); rewrite bijK' -E.
-  rewrite<-(bijK f input). by rewrite->liso_input.
-  rewrite<-(bijK f output). by rewrite->liso_output.
-Defined.
-Instance liso_Equivalence: CRelationClasses.Equivalence liso.
-Proof. constructor. exact @liso_id. exact @liso_sym. exact @liso_comp. Defined.
-
-Lemma iso_liso (G: lgraph) H (h: iso G H): liso G (point H (h input) (h output)).
-Proof. exists (iso_v h) (iso_e h) (fun _ => false)=>//; apply h. Qed.
-
-
-Definition swap Lv (G: graph Lv term_setoid) (f: edge G -> bool): graph Lv term_setoid :=
-  Graph
-    (fun e => if f e then target e else source e)
-    (fun e => if f e then source e else target e)
-    (@vlabel _ _ G)
-    (fun e => if f e then (elabel e)° else elabel e).
-Arguments swap [Lv] G f. 
-
-Definition lswap (G: lgraph) f := point (swap G f) input output. 
-Arguments lswap: clear implicits. 
-
-Lemma swap_liso G f: liso G (lswap G f).
-Proof.
-  liso bij_id bij_id f=>//= e.
-  rewrite /lswap/swap/elabel'/=. case (f e)=>//. apply cnvI. 
-  rewrite /lswap/swap/source'/=. case (f e)=>//. 
-  rewrite /lswap/swap/target'/=. case (f e)=>//.
-Qed.
 
 
 (* TOMOVE *)
@@ -563,19 +281,21 @@ Lemma add_vertex_edge' G w H x y u (l: liso (add_vertex G w) (add_edge H x y u))
   (h x = Some x') * (h y = Some y').
 Admitted.
 
-Definition same_edge (G G' : lgraph) (d : bool) (x : G) (x' : G') (y : G) (y' : G') u u' :
-  if b then [/\ 
+(* Definition same_edge (G G' : lgraph) (l : liso G G') (d : bool) (e : G * term * G) (e' : G' * term * G') := *)
+(*   if b then  *)
+(* (* if b then [/\  *) *)
 
-Definition add_edge_liso' (G G' : lgraph) (l : liso G G') (d : bool) (x : G) (x' : G') (y : G) (y' : G') u u' :
-  same_edge b (x,u,y) (x',u',y') ->
-  liso (G ∔ [x, u, y]) (G' ∔ [x', u', y']).
+(* Definition add_edge_liso' (G G' : lgraph) (l : liso G G') (d : bool) (x : G) (x' : G') (y : G) (y' : G') u u' : *)
+(*   same_edge d (x,u,y) (x',u',y') -> *)
+(*   liso (G ∔ [x, u, y]) (G' ∔ [x', u', y']). *)
+(* Admitted. *)
+
 (* TODO: there is a third case with [u ≡ u'°] *)
-Lemma invert_edge_edge G H x y a b u w (i : liso (add_edge G x y u) (add_edge H a b w)) :
-  (Σ (h : liso G H), (u ≡[i.d None] w) * (i =iso add_edge_liso h
-+ (Σ F a' b' x' y' (g : liso G (add_edge F a' b' w)) (h : liso H (add_edge F x' y' u)), 
-   (g x = x') * (g y = y') * (h a = a') * (h b = b')). (* what else? *)
-Admitted.
-
+(* Lemma invert_edge_edge G H x y a b u w (i : liso (add_edge G x y u) (add_edge H a b w)) : *)
+(*   (Σ (h : liso G H), (u ≡[i.d None] w) * (i =iso add_edge_liso h )) *)
+(* + (Σ F a' b' x' y' (g : liso G (add_edge F a' b' w)) (h : liso H (add_edge F x' y' u)),  *)
+(*    (g x = x') * (g y = y') * (h a = a') * (h b = b')). (* what else? *) *)
+(* Admitted. *)
 
 (* TODO: there is a third case with [u ≡ u'°] *)
 Lemma add_edge_edge G H x y a b u w (i : liso (add_edge G x y u) (add_edge H a b w)) :
@@ -715,6 +435,7 @@ Proof.
       intros (G''&H''&bg&bgh&bh&E). eexists. split. admit. admit.
       (* what about the completely independent case? *)
   - (* pendant rule + chain rule *)
+    rewrite /=. 
     admit.
   - (* pendant rule + loop rule *)
     case: (add_edge_edge h) => [[g] [[A B] C]|].
@@ -752,7 +473,7 @@ Proposition confluence F: forall G H, steps F G -> steps F H -> {F' & steps G F'
 Proof.
   induction F as [F_ IH] using (well_founded_induction_type (Wf_nat.well_founded_ltof _ measure)).
   move=> G H S.
-  move: G H S IH=> _ H [F G FG|F__ F0 G' G FF0 FG GG] IH FH.
+  move: G H S IH => _ H [F G FG|F__ F0 G' G FF0 FG GG] IH FH.
   - exists H; split=>//. transitivity F=>//. by apply liso_step, liso_sym.
   - move: H FH IH FF0=> _ [F H FH|F F1 H' H FF1 FH HH] IH FF0.
     exists G; split=>//. transitivity F. by apply liso_step, liso_sym. eauto using cons_step.
@@ -874,7 +595,9 @@ Admitted.
 
 Lemma par_steps_r G G' H: steps G G' -> steps (lpar H G) (lpar H G').
 Proof.
-  apply step_to_steps. by apply par_liso.
+  apply step_to_steps => {G G'}. by apply par_liso.
+  move => F F'. case.
+  
 Admitted.
 
 Lemma par_steps_l G G' H: steps G G' -> steps (lpar G H) (lpar G' H).
